theories/Prelude/Notations.v
@@ -32,6 +32,7 @@ Reserved Infix "⊆" (no associativity, at level 70).
 
 Reserved Infix "⊢" (no associativity, at level 70).
 Reserved Infix "⊨" (no associativity, at level 70).
+Reserved Infix "⊧" (no associativity, at level 70).
 Reserved Infix "⊬" (no associativity, at level 70).
 Reserved Infix "⊭" (no associativity, at level 70).
 
@@ -56,6 +57,7 @@ Reserved Notation " src '---[' x ']-->*' tgt " (at level 70, no associativity).
 Reserved Notation " src '===[' x ']==>*' tgt " (at level 70, no associativity).
 
 Reserved Notation "Gamma '∋' x '⦂' A" (at level 70, no associativity).
+Reserved Notation "Gamma '⊧' M '⦂' A" (at level 70, no associativity).
 Reserved Notation "Gamma '⊢' M '⦂' A" (at level 70, no associativity).
 Reserved Notation "Gamma '⊢' M '=' N '⦂' A" (at level 70, no associativity).
 Reserved Notation "Gamma '⊢' M '⇉' A" (at level 70, no associativity).
@@ -70,6 +72,7 @@ Reserved Notation "Gamma '⊢' M '~>β' N '⦂' A" (at level 70, no associativit
 Reserved Notation "Gamma '⊢' M '~>η' N '⦂' A" (at level 70, no associativity).
 Reserved Notation "Gamma '⊢' M '~>β*' N '⦂' A" (at level 70, no associativity).
 Reserved Notation "Gamma '⊢' M '~>η*' N '⦂' A" (at level 70, no associativity).
+Reserved Notation "Gamma '⊢' M '~~>' N '⦂' A" (at level 70, no associativity).
 
 Reserved Infix "⟿[  labels  ]" (at level 70, no associativity).
 Reserved Infix "⟿⁺[  labels  ]" (at level 70, no associativity).
